Progress on writing for parser definition.

theories/Parser.v
@@ -2,19 +2,17 @@
 Require Import Coq.Lists.List.
 (* end hide *)
 
-Section Parser.
-
 (** Our parser will be parameterized by a few types and functions that
 determine how it reads data, given in the following record: *)
 
-Record parser_data := ParserData {
+Record parser := Parser {
   state : Type;
   initial_state : state;
   token : state -> Type;
   next : forall s, token s -> state;
   result : state -> Type;
   initial_result : result initial_state;
-  update_result : forall s t, result s -> result (next s t)
+  read_token : forall s, result s -> forall t, result (next s t)
 }.
 
 (** Let's see what each field in this record means.
@@ -35,81 +33,126 @@ Record parser_data := ParserData {
       tells the type of the partial result that our parser has read so
       far. It is initially set to [initial_result], and it is
       incrementally updated with each new token read, using
-      [update_result].
+      [read_token].
 
 Given such data, we can simulate a parsing process ourselves by doing
-successive calls to [update_result]. *)
+successive calls to [read_token]. *)
 
-Variable pd : parser_data.
+Section WithParser.
+
+Variable p : parser.
 
 Definition read_three_tokens t1 t2 t3 :=
-  update_result pd _ t3 (
-    update_result pd _ t2 (
-      update_result pd _ t1 (initial_result pd)
-    )
-  ).
+  read_token p _ (
+    read_token p _ (
+      read_token p _ (initial_result p) t1
+    ) t2
+  ) t3.
 
-(** Needless to say, this is not very convenient for extending Coq's
-syntax. We can make this better by wrapping [parser_data] in another
-type. *)
+(** Needless to say, this is not very convenient as a way of extending
+Coq's syntax. We can make it better by declaring [read_token] as a
+coercion from [result] to [Funclass]. Then, we can read a stream of
+tokens simply by applying [initial_result p] to each token
+successively: *)
 
-Record parser_state (s : state pd) : Type := ParserState {
-  get_result : result pd s
+Coercion read_token : result >-> Funclass.
+
+Definition read_three_tokens' t1 t2 t3 :=
+  (initial_result p) t1 t2 t3.
+
+(** This works because each application of [read_token] returns a
+[result], so trying to apply that updated result to another token
+triggers yet another coercion, allowing the process to continue
+indefinitely. We can check that both definitions of
+[read_three_tokens] yield the same function, meaning that the coercion
+is behaving as expected: *)
+
+Lemma read_three_tokens_same : read_three_tokens = read_three_tokens'.
+Proof. reflexivity. Qed.
+
+(** To make the mechanism more robust, we can wrap our parser in a new
+type, ensuring that the Coq type checker will not fail to perform some
+coercions by reducing [result] more than it should. *)
+
+Record parser_wrapper (s : state p) : Type := ParserWrapper {
+  get_result : result p s
 }.
 
-Definition read_token s (p : parser_state s) t :=
-  ParserState _ (update_result pd s t (get_result s p)).
+Definition read_token' s (w : parser_wrapper s) t :=
+  ParserWrapper _ (read_token p s (get_result s w) t).
+Coercion read_token' : parser_wrapper >-> Funclass.
 
-Definition reader := ParserState _ (initial_result pd).
+End WithParser.
 
-End Parser.
+(** As a last tweak, we declare another coercion and a notation to
+make using our embedded parsers more similar to usual quotations, like
+in Template Haskell: *)
 
-Coercion reader : parser_data >-> parser_state.
-Coercion read_token : parser_state >-> Funclass.
-
+Definition init_parser p := ParserWrapper _ _ (initial_result p).
+Coercion init_parser : parser >-> parser_wrapper.
 Notation "[ x ]" := (get_result _ _ x) (at level 0).
 
-Module List.
+(** Now, we can invoke a parser simply by writing [[name_of_parser
+<list of tokens>]]: *)
 
-Definition p (X : Type) := {|
+Definition read_three_tokens'' (p : parser) t1 t2 t3 :=
+  [p t1 t2 t3].
+
+(** As a first test for our parsing infrastructure, we can define an
+alternative syntax for Coq lists that doesn't need separators between
+the elements. *)
+
+Definition listp (X : Type) := {|
   state := unit;
-  token := fun _ => X;
-  result := fun _ => list X;
   initial_state := tt;
+  token := fun _ => X;
   next := fun _ _ => tt;
+  result := fun _ => list X;
   initial_result := nil;
-  update_result := fun _ x l => app l (cons x nil)
+  read_token := fun _ l x => app l (cons x nil)
 |}.
 
-End List.
+(** The [listp] parser is parameterized by [X], the type of the
+elements on the list. We initialize the parser with an empty list, and
+each token that we read is an element of [X], which will be
+progressively added at the end of our list. *)
 
-Definition my_list : list nat := [List.p _ 1 2 3 4 5 6 7 8 9 10 11].
+Definition my_nat_list : list nat := [listp nat 0 1 2 3 4 5 6 7 8 9 10].
 
-Module Exp.
+(** For [listp], there is no need to use anything interesting for the
+[state] type. For more complicated parsers, however, [state] comes in
+handy. To see how, we will define parsers for prefix and postfix
+arithmetic expressions.
 
-Inductive binop := Plus | Minus | Mult.
+Expressions can involve three operations: addition, subtraction and
+multiplication. *)
 
-Definition ap_binop (b : binop) :=
-  match b with
-  | Plus => plus
-  | Minus => minus
-  | Mult => mult
-  end.
+Inductive op := Add | Sub | Mul.
 
-Inductive inst :=
-| Binop (b : binop)
+(** The expression parsers will read tokens that can be natural
+numbers or one of the above operations. Thus, we group those in a
+common type [exp_token]. *)
+
+Inductive exp_token :=
+| Op (o : op)
 | Const (n : nat).
 
-Module Exports.
+Notation "''+'" := Add (at level 0).
+Notation "''-'" := Sub (at level 0).
+Notation "''*'" := Mul (at level 0).
 
-Notation "''+'" := (Plus) (at level 0).
-Notation "''-'" := (Minus) (at level 0).
-Notation "''*'" := (Mult) (at level 0).
+Coercion Op : op >-> exp_token.
+Coercion Const : nat >-> exp_token.
 
-Coercion Binop : binop >-> inst.
-Coercion Const : nat >-> inst.
+(** To compute the value of an expression, we map each operation to a
+Coq function: *)
 
-End Exports.
+Definition ap_op (o : op) :=
+  match o with
+  | Add => plus
+  | Sub => minus
+  | Mul => mult
+  end.
 
 Module Pre.
 
@@ -119,7 +162,7 @@ Inductive state :=
 
 Definition token (s : state) : Type :=
   match s with
-  | Ok (S _) => inst
+  | Ok (S _) => exp_token
   | _ => Empty_set
   end.
 
@@ -139,21 +182,21 @@ Definition next (s : state) : token s -> state :=
   match s with
   | Ok (S n') => fun t =>
                    match t with
-                   | Binop _ => Ok (S (S n'))
+                   | Op _ => Ok (S (S n'))
                    | Const _ => Ok n'
                    end
   | _ => fun _ => Error
   end.
 
-Definition update_result s : forall t, result s -> result (next s t) :=
+Definition read_token s : result s -> forall t, result (next s t) :=
   match s with
   | Ok (S n') =>
-    fun t =>
+    fun res t =>
       match t with
-      | Binop b => fun res n1 n2 => res (ap_binop b n1 n2)
-      | Const n => fun res => res n
+      | Op o => fun n1 n2 => res (ap_op o n1 n2)
+      | Const n => res n
       end
-  | _ => fun t _ => t
+  | _ => fun _ t => t
   end.
 
 End Pre.
@@ -165,7 +208,7 @@ Definition pre := {|
   result := Pre.result;
   next := Pre.next;
   initial_result := fun t => t;
-  update_result := Pre.update_result
+  read_token := Pre.read_token
 |}.
 
 Module Post.
@@ -178,7 +221,7 @@ Inductive state :=
 Definition token (s : state) : Type :=
   match s with
   | Empty | One => nat
-  | More _ => inst
+  | More _ => exp_token
   end.
 
 Fixpoint result' (n : nat) : Type :=
@@ -200,33 +243,33 @@ Definition next s : token s -> state :=
   | One => fun _ => More 0
   | More 0 => fun t =>
                 match t with
-                | Binop _ => One
+                | Op _ => One
                 | Const _ => More 1
                 end
   | More (S n) => fun t =>
                     match t with
-                    | Binop _ => More n
+                    | Op _ => More n
                     | Const _ => More (S (S n))
                     end
   end.
 
-Definition update_result s : forall t, result s -> result (next s t) :=
+Definition read_token s : result s -> forall t, result (next s t) :=
   match s with
-  | Empty => fun t _ => t
-  | One => fun t r => (r, t)
-  | More 0 => fun t res =>
+  | Empty => fun _ t => t
+  | One => fun res t => (res, t)
+  | More 0 => fun res t =>
                 match res with
                 | (n1, n2) =>
                   match t with
-                  | Binop b => ap_binop b n1 n2
+                  | Op o => ap_op o n1 n2
                   | Const n => (n1, n2, n)
                   end
                 end
-  | More (S n) => fun t res =>
+  | More (S n) => fun res t =>
                     match res with
                     | (res, n1, n2) =>
                       match t with
-                      | Binop b => (res, ap_binop b n1 n2)
+                      | Op o => (res, ap_op o n1 n2)
                       | Const n => (res, n1, n2, n)
                       end
                     end
@@ -241,12 +284,8 @@ Definition post := {|
   initial_state := Post.Empty;
   next := Post.next;
   initial_result := tt;
-  update_result := Post.update_result
+  read_token := Post.read_token
 |}.
 
-End Exp.
-
-Export Exp.Exports.
-
-Definition my_exp : nat := [Exp.pre '+ '- 1 2 '+ 4 4].
-Definition my_exp' : nat := [Exp.post 4 4 '+ 2 1 '- '+].
+Definition my_exp : nat := [pre '+ '- 1 2 '+ 4 4].
+Definition my_exp' : nat := [post 4 4 '+ 2 1 '- '+].
